Cleanup and rebalancing
	modified:   src/.gitignore
	modified:   src/Avl_tree.v
	modified:   src/Binary_search_tree.v
	modified:   src/Binary_tree.v

src/Avl_tree.v
@@ -34,6 +34,13 @@ Module Make (S0:SORTABLE).
       | _ => False
       end.
 
+
+    Definition Leaning (b:T): Prop :=
+      match b with
+      | left | right => True
+      | balanced => False
+      end.
+
     Theorem left_not_balanced: left <> balanced.
     Proof
       fun eq => Equal.rewrite eq Left I.
@@ -65,6 +72,7 @@ Module Make (S0:SORTABLE).
   Definition Left_leaning  (t:T): Prop := Extra t B.left.
   Definition Right_leaning (t:T): Prop := Extra t B.right.
   Definition Balanced (t:T): Prop := Extra t B.balanced.
+  Definition Leaning (t:T): Prop := Left_leaning t \/ Right_leaning t.
 
 
   Theorem left_leaning_is_node:
@@ -78,9 +86,18 @@ Module Make (S0:SORTABLE).
     fun t bal => extra_is_node bal.
 
   Theorem right_leaning_is_node:
-    forall (t:T), Balanced t -> Node t.
+    forall (t:T), Right_leaning t -> Node t.
   Proof
     fun t bal => extra_is_node bal.
+
+  Theorem leaning_is_node:
+    forall t:T, Leaning t -> Node t.
+  Proof
+    fun t leaning =>
+      match leaning with
+      | or_introl p => left_leaning_is_node p
+      | or_intror p => right_leaning_is_node p
+      end.
 
   Inductive Avl_height: T -> nat -> Prop :=
   | empty_avl: Avl_height empty 0
@@ -103,872 +120,149 @@ Module Make (S0:SORTABLE).
   Definition Avl_tree (t:T): Prop :=
     exists h, Avl_height t h.
 
+  Theorem avl_height_positive_is_node:
+    forall (t:T) (h:nat),
+      Avl_height t (S h) ->
+      Node t.
+  Proof
+    let f t h_ (avl:Avl_height t h_): forall h, S h = h_  -> Node t :=
+      (match avl in Avl_height t h_
+            return forall h, S h = h_ -> Node t with
+      | empty_avl =>
+        fun h eq => match Nat.successor_not_zero eq with end
+      | @balanced_avl h a t1 t2 ph1 ph2 =>
+        fun _ _ => I
+      | @left_avl h a t1 t2 ph1 ph2 =>
+        fun _ _ => I
+      | @right_avl h a t1 t2 ph1 ph2 =>
+        fun _ _ => I
+      end)
+    in
+    fun t h avl => f t (S h) avl h eq_refl .
+
+
+
 
   (*====================================*)
   (** * Rebalancing *)
   (*====================================*)
 
-  (** An avl tree is nearly balanced if its left and right subtree differ in
-      height by not more than 2. *)
-
-  Inductive Nearly_avl_left: A -> B.T -> T -> T -> nat -> Prop :=
-  | ok_nearly_left:
-      forall a bal t1 t2 h,
-        Avl_height (node a bal t1 t2) h ->
-        Nearly_avl_left a bal t1 t2 h
-  | left_nearly_left:
-      forall h t1 t2 a,
-        Avl_height t1 (2+h) ->
-        Avl_height t2 h ->
-        Nearly_avl_left  a B.left t1 t2 (3+h).
-
-  Inductive Nearly_avl_right: T -> nat -> Prop :=
-  | avl_nearly_right:
-      forall t h,
-        Avl_height t h ->
-        Nearly_avl_right t h
-  | right_nearly_right:
-      forall h t1 t2 a,
-        Avl_height t1 h ->
-        Avl_height t2 (2+h) ->
-        Nearly_avl_right (node a B.right t1 t2) (3+h).
-
-
-  Inductive Rebalanced_left: A -> B.T -> T -> T -> T -> nat -> Prop :=
-  | l_rebalanced:
-      (* No rebalancing
+  Inductive Nearly_avl_left: A -> T -> T -> Prop :=
+  | lrl_nearly_avl_left:
+      (* lrl:
+                      c
+              a            t2
+          t11     b        x
+          x   t121 t122
+              x
        *)
-      forall a bal t1 t2 h,
-        Avl_height (node a bal t1 t2) h ->
-        Rebalanced_left a bal t1 t2 (node a bal t1 t2) h
-  | ll_rebalanced:
-      (*
-                    b                            a
-              a          t3              t1             b
-          t1     t2                      x          t2      t3
+      forall h t11 t121 t122 t2 a b c,
+        Avl_height t11 (1+h) ->
+        Avl_height t121 (1+h) ->
+        Avl_height t122 h ->
+        Avl_height t2 (1+h) ->
+        Nearly_avl_left
+          c
+          (node a B.right t11 (node b B.left t121 t122))
+          t2
+  | lrr_nearly_avl_left:
+      (* lrl:
+                      c
+              a            t2
+          t11     b        x
+          x   t121 t122
+                   x
+       *)
+      forall h t11 t121 t122 t2 a b c,
+        Avl_height t11 (1+h) ->
+        Avl_height t121 h ->
+        Avl_height t122 (1+h) ->
+        Avl_height t2 (1+h) ->
+        Nearly_avl_left
+          c
+          (node a B.right t11 (node b B.right t121 t122))
+          t2
+  | ll_nearly_avl_left:
+      (* ll:
+                    c
+              a          t2
+          t11    t12
           x
        *)
-      forall h t1 t2 t3 a b bal,
-        Avl_height t1 (1+h) ->
-        Avl_height t2 h ->
-        Avl_height t3 h ->
-        Rebalanced_left
-          b bal (node a B.left t1 t2) t3
-          (node a B.balanced t1 (node b B.balanced t2 t3))
-          (2+h)
-  | lrl_rebalanced:
-      (*
+      forall h t11 t12 t2 a c,
+        Avl_height t11 (1+h) ->
+        Avl_height t12 h ->
+        Avl_height t2  h ->
+        Nearly_avl_left
+          c
+          (node a B.left t11 t12)
+          t2.
+
+
+
+
+  Definition rebalance_left (c:A) (t1 t2:T): T :=
+    match t1  with
+    | empty =>
+      node c B.right empty t2
+    | node a B.right t11 (node b B.left t121 t122) =>
+      (* lrl:
                       c                               b
-              a            t4                   a            c
-          t1     b         x                 t1   t2      t3   t4
-          x   t2  t3                         x    x            x
+              a            t2                   a            c
+          t11     b        x                 t11  t121   t122  t2
+          x   t121 t122                      x    x            x
               x
        *)
-      forall h t1 t2 t3 t4 a b c bal,
-        Avl_height t1 (1+h) ->
-        Avl_height t2 (1+h) ->
-        Avl_height t3 h ->
-        Avl_height t4 (1+h) ->
-        Rebalanced_left
-          c
-          bal
-          (node a B.right
-                t1
-                (node b B.left t2 t3))
-          t4
-          (node b B.balanced
-                (node a B.balanced t1 t2)
-                (node c B.right t3 t4))
-          (3+h)
-  | lrr_rebalanced:
-      (*
+      node
+        b B.balanced
+        (node a B.balanced t11 t121)
+        (node c B.right t122 t2)
+    | node a B.right t11 (node b B.right t121 t122) =>
+      (* lrr:
                       c                               b
-              a            t4                   a            c
-          t1     b         x                 t1   t2      t3   t4
-          x   t2  t3                         x            x    x
-                  x
+              a            t2                   a            c
+          t11     b        x                 t11  t121   t122  t2
+          x   t121 t122                      x           x     x
+                   x
        *)
-      forall h t1 t2 t3 t4 a b c bal,
-        Avl_height t1 (1+h) ->
-        Avl_height t2 h ->
-        Avl_height t3 (1+h) ->
-        Avl_height t4 (1+h) ->
-        Rebalanced_left
-          c
-          bal
-          (node a B.right
-                t1
-                (node b B.right t2 t3))
-          t4
-          (node b B.balanced
-                (node a B.left t1 t2)
-                (node c B.balanced t3 t4))
-          (3+h).
-
-  Theorem rebalanced_left_correct:
-    forall (a:A) (bal:B.T) (t1 t2 t3:T) (h:nat),
-      Rebalanced_left a bal t1 t2 t3 h ->
-      Avl_height t3 h.
-  Proof
-    fun a bal t1 t2 t3 h rebal =>
-      match rebal in Rebalanced_left a bal t1 t2 t3 h
-            return Avl_height t3 h
-      with
-      | @l_rebalanced a bal t1 t2 h pheight =>
-        pheight
-      | @ll_rebalanced h t1 t2 t3 a b bal pt1 pt2 pt3 =>
-        @balanced_avl
-          (1+h) a t1 (node b B.balanced t2 t3)
-          pt1
-          (@balanced_avl h b t2 t3 pt2 pt3)
-      | @lrl_rebalanced h t1 t2 t3 t4 a b c bal pt1 pt2 pt3 pt4 =>
-        @balanced_avl
-          (2+h) b _ _
-          (@balanced_avl (1+h) a t1 t2 pt1 pt2)
-          (@right_avl h c t3 t4 pt3 pt4)
-      | @lrr_rebalanced h t1 t2 t3 t4 a b c bal pt1 pt2 pt3 pt4 =>
-        @balanced_avl
-          (2+h) b _ _
-          (@left_avl h a t1 t2 pt1 pt2)
-          (@balanced_avl (1+h) c t3 t4 pt3 pt4)
-      end.
-
-
-  Definition rebalance_left (x:A) (xbal:B.T) (u v:T): T :=
-    match u with
-    | node a B.left t1 t2 =>
-      (* ll *)
-      node a B.balanced t1 (node x B.balanced t2 v)
-    | node a B.right t1 (node b B.left t2 t3) =>
-      (* lrl *)
-      node b B.balanced
-           (node a B.balanced t1 t2)
-           (node x B.right t3 v)
-
-    | node a B.right t1 (node b B.right t2 t3) =>
-      (* lrr *)
-      node b B.balanced
-           (node a B.left t1 t2)
-           (node x B.balanced t3 v)
-
-    | _ =>
-      node x xbal u v
+      node
+        b B.balanced
+        (node a B.left t11 t121)
+        (node c B.balanced t122 t2)
+    | node a bal t11 t12 =>
+      (* ll:
+                    c                            a
+              a          t2              t11            c
+          t11    t12                     x          t12   t2
+          x
+       *)
+      node a B.balanced t11 (node c B.balanced t12 t2)
     end.
 
-(*
-  Theorem rebalance_left_correct:
-    forall (a:A) (bal:B.T) (t1 t2 t3:T) (h:nat),
-      Rebalanced_left a bal t1 t2 t3 h ->
-      t3 = rebalance_left a bal t1 t2.
+
+  Theorem rebalance_left_rebalances:
+    forall (a:A) (t1 t2:T) (nearly:Nearly_avl_left a t1 t2),
+      Avl_tree (rebalance_left a t1 t2).
   Proof
-    _
-  .
-*)
+    fun a t1 t2 nearly =>
+      match nearly in Nearly_avl_left a t1 t2
+            return Avl_tree (rebalance_left a t1 t2)
+      with
+      | lrl_nearly_avl_left a b c ph11 ph121 ph122 ph2 =>
+        let pa := balanced_avl a ph11 ph121 in
+        let pc := right_avl c ph122 ph2 in
+        let pb := balanced_avl b pa pc in
+        ex_intro _ _ pb
+      | lrr_nearly_avl_left a b c ph11 ph121 ph122 ph2 =>
+        let pa := left_avl a ph11 ph121 in
+        let pc := balanced_avl c ph122 ph2 in
+        let pb := balanced_avl b pa pc in
+        ex_intro _ _ pb
+      | ll_nearly_avl_left a c ph11 ph12 ph2 =>
+        let pc := balanced_avl c ph12 ph2 in
+        let pa := balanced_avl a ph11 pc in
+        ex_intro _ _ pa
+      end.
 
-
-
-
-
-  Inductive Rebalanced_right: T -> T -> Prop :=
-  | r_rebalanced:
-      forall t h,
-        Avl_height t h ->
-        Rebalanced_right t t
-  (*
-              a                                     b
-        t1          b                         a          t3
-                 t2   t3                   t1   t2       x
-                      x
-   *)
-  | rr_rebalanced:
-      forall h t1 t2 t3 a b bal,
-        Avl_height t1 h ->
-        Avl_height t2 h ->
-        Avl_height t3 (1+h) ->
-        Rebalanced_right
-          (node a bal t1 (node b B.right t2 t3))
-          (node b B.balanced (node a B.balanced t1 t2) t3)
-  (*
-              a                                     b
-        t1            c                       a            c
-        x        b       t4                t1   t2      t3   t4
-              t2   t3    x                 x    x            x
-              x
-   *)
-  | rll_rebalanced:
-      forall h t1 t2 t3 t4 a b c bal,
-        Avl_height t1 (1+h) ->
-        Avl_height t2 (1+h) ->
-        Avl_height t3 h ->
-        Avl_height t4 (1+h) ->
-        Rebalanced_right
-          (node a bal
-                t1
-                (node c B.left
-                      (node b B.left t2 t3)
-                      t4))
-          (node b B.balanced
-             (node a B.balanced t1 t2)
-             (node c B.right t3 t4))
-  (*
-              a                                     b
-        t1            c                       a            c
-        x        b       t4                t1   t2      t3   t4
-              t2   t3    x                 x            x    x
-                   x
-   *)
-  | rlr_rebalanced:
-      forall h t1 t2 t3 t4 a b c bal,
-        Avl_height t1 (1+h) ->
-        Avl_height t2 h ->
-        Avl_height t3 (1+h) ->
-        Avl_height t4 (1+h) ->
-        Rebalanced_right
-          (node a bal
-                t1
-                (node c B.left
-                      (node b B.right t2 t3)
-                      t4))
-          (node b B.balanced
-             (node a B.left t1 t2)
-             (node c B.balanced t3 t4)).
 
 End Make.
-
-
-
-
-Module Make2 (S:SORTABLE).
-  Import Relation.
-
-(** * Sortable *)
-(*    ======== *)
-  Module S1 := Sortable_plus S.
-  Section sortable.
-
-    Definition A:Set :=  S1.T.
-
-    Definition dichotomic := S1.dichotomic.
-    Definition transitive := S1.transitive.
-    Definition reflexive  := S1.reflexive.
-
-  End sortable.
-  Notation "a <= b"  := (S.Less_equal a b) (at level 70).
-  Notation "a <=? b" := (S.is_less_equal a b) (at level 70).
-  Notation "( 'transitivity_chain:' x , y , .. , z )" :=
-    (transitive .. (transitive x y) .. z) (at level 0).
-
-
-  Definition Equivalent (a b:A): Prop := a <= b /\ b <= a.
-
-
-
-(** * List *)
-(*    ==== *)
-  Module List.
-    Definition L: Set := list A.
-
-    Inductive Permutation: L -> L -> Prop :=
-    | perm_empty:
-        Permutation [] []
-    | perm_prefix:
-        forall x a b, Permutation a b -> Permutation (x::a) (x::b)
-    | perm_swap:
-        forall x y a,  Permutation (x::y::a) (y::x::a)
-    | perm_transitive:
-        forall a b c,  Permutation a b -> Permutation b c -> Permutation a c.
-  End List.
-
-
-
-(** * Basic Definitions *)
-(*    ================= *)
-  Section basic_definitions.
-    Inductive Balance: Set :=
-      balanced: Balance
-    | left_leaning: Balance.
-
-    Inductive T :=
-      empty: T
-    | node:  Balance -> A -> T -> T -> T.
-
-    Fixpoint height (t:T): nat :=
-      match t with
-      | empty => 0
-      | node _ _ t1 t2 => 1 + max (height t1) (height t2)
-      end.
-
-    Definition Node (t:T): Prop :=
-      match t with
-      | empty => False
-      | node _ _ _ _ => True
-      end.
-
-    Inductive Domain: T -> A -> Prop :=
-    | domain_node:
-        forall x b a t1 t2,
-          x = a -> Domain (node b a t1 t2) x
-    | domain_left:
-        forall x a b t1 t2,
-          Domain t1 x -> Domain (node b a t1 t2) x
-    | domain_right:
-        forall x a b t1 t2,
-          Domain t2 x -> Domain (node b a t1 t2) x.
-
-
-    Theorem node_not_empty:
-      forall (b:Balance) (a:A) (t1 t2: T),
-        node b a t1 t2 <> empty.
-    Proof
-      fun b a t1 t2 p =>
-        Equal.rewrite p Node I.
-
-    Definition is_node (t:T): {Node t} + {~ Node t} :=
-      match t return {Node t} + {~ Node t} with
-        empty => right (fun p:False => match p with end)
-      | node b a t1 t2 => left I
-      end.
-
-    Definition element (t:T): Node t -> A :=
-      match t return Node t -> A with
-      | empty => fun p:Node empty => match p with end
-      | node _ a _ _ => fun _ => a
-      end.
-
-    Definition left_son (t:T): Node t -> T :=
-      match t return Node t -> T with
-      | empty => fun p:Node empty => match p with end
-      | node _ _ t1 _ => fun _ => t1
-      end.
-
-    Definition right_son (t:T): Node t -> T :=
-      match t return Node t -> T with
-      | empty => fun p:Node empty => match p with end
-      | node _ _ _ t2 => fun _ => t2
-      end.
-
-
-    Definition balance (t:T): Balance :=
-      match t with
-      | empty => balanced
-      | node b _ _ _ => b
-      end.
-
-    Fixpoint least (t:T): Node t -> A :=
-      match t return Node t -> A with
-      | empty =>
-        fun p => match p with end
-      | node b a t1 t2 =>
-        match is_node t1 with
-          left  pt1 => fun _ => least t1 pt1
-        | right pt1 => fun _ => a
-        end
-      end.
-
-    Fixpoint greatest (t:T): Node t -> A :=
-      match t return Node t -> A with
-      | empty =>
-        fun p => match p with end
-      | node b a t1 t2 =>
-        match is_node t2 with
-          left  pt2 => fun _ => greatest t2 pt2
-        | right pt2 => fun _ => a
-        end
-      end.
-  End basic_definitions.
-
-
-(** * Module 'Node' Describing the Content of a Node *)
-(*    ============================================== *)
-  Module Node.
-    Import Equal.Notations.
-    Record N := make { balance:Balance; element:A; left:T; right:T}.
-
-    Definition Tree_node (n:N) (t:T): Prop :=
-      t = node n.(balance) n.(element) n.(left) n.(right).
-
-    Definition tree_node (t:T): Node t -> {n:N | Tree_node n t} :=
-      match t return Node t -> {n | Tree_node n t} with
-      | empty =>
-        fun p => match p with end
-      | node b a t1 t2 =>
-        fun _ =>
-          let n := make b a t1 t2 in
-          let p: Tree_node n (node b a t1 t2) :=
-              (equal_arguments: eq_refl, eq_refl, eq_refl, eq_refl)
-          in
-          exist _ n p
-      end.
-  End Node.
-
-
-(** * Balanced Trees *)
-(*    ============== *)
-  Section balanced.
-    Inductive Balanced: nat -> Balance -> T -> Prop :=
-      balanced_empty:
-        Balanced 0 balanced empty
-    | balanced_perfect:
-        forall h b1 t1 b2 t2 h_new a,
-          h_new = 1 + h ->
-          Balanced h b1 t1 ->
-          Balanced h b2 t2 ->
-          Balanced h_new balanced (node balanced a t1 t2)
-    | balanced_left_leaning:
-        forall h1 b1 t1 h2 b2 t2 h_new a,
-          h1 = 1 + h2 ->
-          h_new = 2 + h2 ->
-          Balanced h1 b1 t1 ->
-          Balanced h2 b2 t2 ->
-          Balanced h_new left_leaning (node left_leaning a t1 t2).
-
-    Definition Balanced_tree (t:T): Prop :=
-      Balanced (height t) (balance t) t.
-
-
-    Inductive Balanced2: nat -> T -> Prop :=
-    | bal_empty: Balanced2 0 empty
-    | bal_equal: forall h t1 t2 a,
-        Balanced2 h t1 ->
-        Balanced2 h t2 ->
-        Balanced2 (1+h) (node balanced a t1 t2)
-    | bal_left: forall h t1 t2 a,
-        Balanced2 (1+h) t1 ->
-        Balanced2 h t2 ->
-        Balanced2 (2+h) (node left_leaning a t1 t2).
-
-
-    Theorem height_consistent2:
-      forall (h:nat) (t:T), Balanced2 h t -> h = height t.
-    Proof
-      fix f h t p {struct p}: h = height t :=
-      (* height (node _ _ t1 t2) = 1 + max (height t1) (height t2)
-       *)
-      match p in Balanced2 h t return h = height t with
-      | bal_empty =>
-        eq_refl
-      | @bal_equal h t1 t2 a bal1 bal2 =>
-        (equality_chain:
-           (eq_refl: 1 + h = _)
-           ,
-           (let p : max h h = h := max_l h h (le_n h) in
-            Equal.inject (Equal.flip p) (fun x => 1 + x)
-            : _ = 1 + max h h)
-           ,
-           (let ht1: h = height t1 := f h t1 bal1 in
-            Equal.inject ht1 (fun x => 1 + max x h)
-            : _ = 1 + max (height t1) h)
-           ,
-           (let ht2: h = height t2 := f h t2 bal2 in
-            Equal.inject ht2 (fun x => 1 + max (height t1) x)
-            : _ = 1 + max (height t1) (height t2))
-           ,
-           (eq_refl: _ = height (node balanced a t1 t2))
-        )
-      | @bal_left h t1 t2 a bal1 bal2 =>
-        (equality_chain:
-           (eq_refl: 2 + h = _)
-           ,
-           (let p: max (1+h) h = 1 + h := max_l (1+h) h (le_S _ h (le_n h)) in
-            Equal.inject (Equal.flip p) (fun x => 1 + x)
-            : _ = 1 + max (1+h) h)
-           ,
-           (let ht1: 1 + h = height t1 := f (1+h) t1 bal1 in
-            Equal.inject ht1 (fun x => 1 + max x h)
-            : _ = 1 + max (height t1) h)
-           ,
-           (let ht2: h = height t2 := f h t2 bal2 in
-            Equal.inject ht2 (fun x => 1 + max (height t1) x)
-            : _ = 1 + max (height t1) (height t2))
-           ,
-           (eq_refl: _ = height (node left_leaning a t1 t2))
-        )
-      end.
-
-
-    Theorem height_consistent:
-      forall (h:nat) (b:Balance) (t:T), Balanced h b t -> h = height t.
-    Proof.
-      refine(
-      fix f h b t p {struct p}: h = height t  :=
-        match p in Balanced h b t return h = height t with
-        | balanced_empty => eq_refl
-        | @balanced_perfect h b1 t1 b2 t2 h_new a ph p1 p2 =>
-          let pht1: h = height t1 := f h b1 t1 p1 in
-          let pht2: h = height t2 := f h b2 t2 p2 in
-          _
-        | @balanced_left_leaning h1 b1 t1 h2 b2 t2 h_new a ph1 ph_new p1 p2 =>
-          let pht1: h1 = height t1 := f h1 b1 t1 p1 in
-          let pht2: h2 = height t2 := f h2 b2 t2 p2 in
-          _
-        end).
-      - simpl. rewrite <- pht1. rewrite <- pht2.
-        rewrite max_l. assumption. apply le_n.
-      - simpl. rewrite <- pht1. rewrite <- pht2.
-        rewrite max_l. rewrite ph_new. rewrite ph1. reflexivity.
-        rewrite ph1. apply le_S. apply le_n.
-    Qed.
-
-    Theorem balanced_is_balanced_tree:
-      forall (h:nat) (b:Balance) (t:T),
-        Balanced h b t ->
-        Balanced_tree t.
-    Proof.
-      refine (
-          fix f h b t pbal :=
-            match pbal in Balanced h b t return Balanced_tree t with
-            | balanced_empty =>
-              balanced_empty
-            | @balanced_perfect
-                h b1 t1 b2 t2 h_new a
-                ph pbal1 pbal2 =>
-              let ph1: h = height t1 := @height_consistent h b1 t1 pbal1 in
-              let ph2: h = height t2 := @height_consistent h b2 t2 pbal2 in
-              _
-            | @balanced_left_leaning
-                h1 b1 t1 h b2 t2 h_new a
-                ph1 phnew pbal1 pbal2 =>
-              let pht1: h1 = height t1 := @height_consistent h1 b1 t1 pbal1 in
-              let pht2: h  = height t2 := @height_consistent h  b2 t2 pbal2 in
-              _
-            end).
-      - unfold Balanced_tree. simpl. rewrite <- ph1. rewrite <- ph2. rewrite max_l.
-        apply balanced_perfect with (h:=h)(b1:=b1)(b2:=b2).
-        reflexivity. assumption. assumption. apply le_n.
-      - unfold Balanced_tree.  simpl. rewrite <- pht1. rewrite <- pht2.
-        rewrite max_l.
-        apply balanced_left_leaning with (h1:=h1) (b1:=b1) (h2:=h) (b2:=b2).
-        assumption. rewrite ph1. reflexivity. assumption. assumption.
-        rewrite ph1. apply le_S. apply le_n.
-    Qed.
-
-    Theorem balanced_subtree:
-      forall (b:Balance) (h:nat) (t:T),
-        Balanced h b t ->
-        forall p:Node t,
-          Balanced_tree (left_son t p) /\
-          Balanced_tree (right_son t p).
-    Proof
-      fun b h t pbal =>
-        match pbal in Balanced h b t
-              return
-              forall p:Node t,
-                Balanced_tree (left_son t p) /\
-                Balanced_tree (right_son t p)
-        with
-        | balanced_empty =>
-          fun pnode => match pnode with end
-        | @balanced_perfect h b1 t1 b2 t2 h_new a ph pbal1 pbal2 =>
-          fun pnode =>
-            let lson := left_son  (node balanced a t1 t2) pnode in
-            let rson := right_son (node balanced a t1 t2) pnode in
-            let peq1 : t1 = lson := eq_refl in
-            let peq2 : t2 = rson := eq_refl in
-            let pbal_left: Balanced h b1 lson :=
-                Equal.rewrite peq1 (Balanced h b1) pbal1 in
-            let pbal_right: Balanced h b2 rson :=
-                Equal.rewrite peq2 (Balanced h b2) pbal2 in
-            conj
-              (@balanced_is_balanced_tree h b1 lson pbal_left)
-              (@balanced_is_balanced_tree h b2 rson pbal_right)
-        | @balanced_left_leaning h1 b1 t1 h b2 t2 h_new a ph1 phnew pbal1 pbal2 =>
-          fun pnode =>
-            let lson := left_son  (node left_leaning a t1 t2) pnode in
-            let rson := right_son (node left_leaning a t1 t2) pnode in
-            let peq1 : t1 = lson := eq_refl in
-            let peq2 : t2 = rson := eq_refl in
-            let pbal_left: Balanced h1 b1 lson :=
-                Equal.rewrite peq1 (Balanced h1 b1) pbal1 in
-            let pbal_right: Balanced h b2 rson :=
-                Equal.rewrite peq2 (Balanced h b2) pbal2 in
-            conj
-              (@balanced_is_balanced_tree h1 b1 lson pbal_left)
-              (@balanced_is_balanced_tree h  b2 rson pbal_right)
-        end.
-  End balanced.
-
-
-
-(** * Sorted Trees *)
-(*    ============ *)
-  Section sorted.
-    Inductive Sorted: A -> A -> T -> Prop :=
-      empty_sorted:
-        forall lo hi, lo <= hi -> Sorted lo hi empty
-    | node_sorted:
-        forall lo1 hi1 t1 lo2 hi2 t2 b a,
-          Sorted lo1 hi1 t1 ->
-          Sorted lo2 hi2 t2 ->
-          hi1 <= a ->
-          a <= lo2 ->
-          Sorted lo1 hi2 (node b a t1 t2).
-
-    Theorem bounds_sorted:
-      forall (lo hi:A) (t:T),
-        Sorted lo hi t -> lo <= hi.
-    Proof
-      fix f lo hi t s :=
-      match s in Sorted lo hi t return lo <= hi with
-      | @empty_sorted lo hi p => p
-      | @node_sorted lo1 hi1 t1 lo2 hi2 t2 b a s1 s2 le1 le2 =>
-        let p1: lo1 <= hi1 := f lo1 hi1 t1 s1 in
-        let p2: lo2 <= hi2 := f lo2 hi2 t2 s2 in
-        (transitivity_chain: p1, le1, le2, p2)
-      end.
-
-    Theorem bounds_extendible:
-      forall (lo lo0 hi0 hi:A) (t:T),
-        Sorted lo0 hi0 t ->
-        lo <= lo0 ->
-        hi0 <= hi ->
-        Sorted lo hi t.
-    Proof
-      fix f lo lo0 hi0 hi t s :=
-      match s in Sorted lo0 hi0 t
-            return lo <= lo0 -> hi0 <= hi -> Sorted lo hi t with
-      | @empty_sorted lo0 hi0 p =>
-        fun (le1:lo<=lo0) (le2:hi0<=hi) =>
-          @empty_sorted
-            lo hi
-            (transitivity_chain: le1, p, le2)
-      | @node_sorted lo1 hi1 t1 lo2 hi2 t2 b a
-                     s1 s2 le_hi1_a le_a_lo2 =>
-        fun (le1:lo<=lo1) (le2:hi2<=hi) =>
-          let p1: Sorted lo hi1 t1 :=
-              f lo lo1 hi1 hi1 t1 s1 le1 (reflexive hi1)
-          in
-          let p2: Sorted lo2 hi t2 :=
-              f lo2 lo2 hi2 hi t2 s2 (reflexive lo2) le2
-          in
-          @node_sorted lo hi1 t1 lo2 hi t2 b a p1 p2 le_hi1_a le_a_lo2
-      end.
-
-
-
-    Definition Sorted_tree (t:T): Prop :=
-      match is_node t with
-      | left  p => (* p: Node t *)
-        Sorted (least t p) (greatest t p) t
-      | right p => (* p: ~ Node t *)
-        True
-      end.
-
-    Definition Sorted_tree2 (t:T): Prop :=
-      exists lo hi, Sorted lo hi t.
-
-    Theorem least_is_infimum:
-      forall (lo hi:A) (t:T),
-        Sorted lo hi t -> forall nd:Node t, lo <= least t nd.
-    Proof
-      let Cond lo t nd := lo <= least t nd
-      in
-      fix f lo hi t sorted :=
-      match sorted in Sorted lo hi t
-            return forall nd, Cond lo t nd
-      with
-      | empty_sorted _ =>
-        fun nd =>
-          match nd with end
-      | @node_sorted lo1 hi1 t1
-                     lo2 hi2 t2
-                     b a
-                     s1 s2 le_l_a le_a_r =>
-        fun nd =>
-          (match
-              t1
-              return (forall nd, Cond lo1 t1 nd) ->
-                     Cond lo1 (node b a t1 t2) nd
-           with
-           | empty =>
-             fun _ =>
-               Equal.rewrite
-                 (eq_refl : a = least (node b a empty t2) nd)
-                 (fun x => lo1 <= x)
-                 ((transitivity_chain: bounds_sorted s1, le_l_a): lo1 <= a)
-           | node b1 a1 t11 t12 =>
-             let t_ := node b1 a1 t11 t12 in
-             fun p1: forall nd1, Cond lo1 t_ nd1 =>
-               p1 I
-           end) (f lo1 hi1 t1 s1)
-      end.
-
-    Theorem least_is_least:
-      forall (lo hi:A) (t:T),
-        Sorted lo hi t ->
-        forall nd:Node t,
-          lo <= least t nd /\ Sorted (least t nd) hi t.
-    Proof
-      let Cond lo hi t nd :=
-          lo <= least t nd /\ Sorted (least t nd) hi t
-      in
-      fix f lo hi t sorted :=
-      match sorted in Sorted lo hi t
-            return forall nd, Cond lo hi t nd
-      with
-      | empty_sorted _ =>
-        fun nd =>
-          match nd with end
-      | @node_sorted lo1 hi1 t1
-                     lo2 hi2 t2
-                     b a
-                     s1 s2 le_hi1_a le_a_lo2 =>
-        fun nd =>
-          (match
-              t1
-              return (forall nd, Cond lo1 hi1 t1 nd) ->
-                     Cond lo1 hi2 (node b a t1 t2) nd
-           with
-           | empty =>
-             fun p1 =>
-               let t_ := node b a empty t2 in
-               Equal.rewrite
-                 (eq_refl : a = least t_ nd)
-                 (fun x => lo1 <= x /\ Sorted x hi2 t_)
-                 (conj
-                    ((transitivity_chain: bounds_sorted s1, le_hi1_a):lo1 <= a)
-                    (@node_sorted
-                       a a empty lo2 hi2 t2 b a
-                       (empty_sorted (reflexive a))
-                       s2
-                       (reflexive a)
-                       le_a_lo2
-                     : Sorted (least t_ nd) hi2 t_)
-                 )
-           | node b1 a1 t11 t12 =>
-             let t_ := node b1 a1 t11 t12 in
-             fun p1: forall nd1, Cond lo1 hi1 t_ nd1 =>
-               let p11: lo1 <= least t_ I  :=
-                   proj1 (p1 I) in
-               let p12: Sorted (least t_ I) hi1 t_
-                   := proj2 (p1 I) in
-               conj
-                 p11
-                 (@node_sorted
-                    (least t_ I) hi1 t_ lo2 hi2 t2 b a
-                    p12
-                    s2
-                    le_hi1_a
-                    le_a_lo2
-                 )
-            end) (f lo1 hi1 t1 s1)
-      end.
-
-
-    Theorem greatest_is_supremum:
-      forall (lo hi:A) (t:T),
-        Sorted lo hi t -> forall nd:Node t, greatest t nd <= hi.
-    Proof
-      let Cond hi t := forall nd:Node t, greatest t nd <= hi
-      in
-      fix f lo hi t sorted :=
-      match sorted in Sorted lo hi t
-            return Cond hi t
-      with
-      | empty_sorted _ =>
-        fun nd =>
-          match nd with end
-      | @node_sorted lo1 hi1 t1
-                     lo2 hi2 t2
-                     b a
-                     s1 s2 le_l_a le_a_r =>
-        fun nd =>
-          (match
-              t2
-              return (Cond hi2 t2) -> greatest (node b a t1 t2) nd <= hi2
-           with
-           | empty =>
-             fun _ =>
-               Equal.rewrite
-                 (eq_refl : a = greatest (node b a t1 empty) nd)
-                 (fun x => x <= hi2)
-                 (* a <= lo2 <= hi2 *)
-                 (transitivity_chain: le_a_r, bounds_sorted s2)
-           | node b2 a2 t21 t22 =>
-             let t := node b2 a2 t21 t22 in
-             fun p1: forall nd2,
-                 greatest t nd2 <= hi2 =>
-               p1 I
-           end) (f lo2 hi2 t2 s2)
-      end.
-
-
-    Theorem root_element_sorted:
-      forall (t:T) (lo hi:A),
-        Sorted lo hi t ->
-        forall (nd:Node t),
-          lo <= element t nd /\ element t nd <= hi.
-    Proof
-      (* match sorted:
-         a) empty: by contradiction
-         b) node:  lo1 <= hi1  (bounds_sorted)
-                   hi1 <= a    (Sorted ...)
-                   a = element t nd
-                   a <= lo2    (Sorted ...)
-                   lo2 <= hi2  (bounds_sorted)
-       *)
-      let Cond lo hi t nd :=
-          lo <= element t nd /\ element t nd <= hi
-      in
-      fun t lo hi sorted =>
-        match sorted in Sorted lo hi t
-              return forall nd, Cond lo hi t nd
-        with
-        | empty_sorted _ =>
-          fun nd =>
-            match nd with end
-        | @node_sorted lo1 hi1 t1
-                       lo2 hi2 t2
-                       b a
-                       s1 s2 le_hi1_a le_a_lo2 =>
-          (* goal: forall nd: Node (node b a t1 t2),
-                      lo1 <= element (node b a t1 t2) nd *)
-          fun nd =>
-            let eq_a: a = element (node b a t1 t2) nd := eq_refl in
-            conj
-              (Equal.rewrite
-                 eq_a
-                 (fun x => lo1 <= x)
-                 (transitivity_chain: bounds_sorted s1,le_hi1_a))
-              (Equal.rewrite
-                 eq_a
-                 (fun x => x <= hi2)
-                 (transitivity_chain: le_a_lo2, bounds_sorted s2))
-        end.
-
-  End sorted.
-
-  Section draft.
-
-
-    (* Replace a t1 t2: An element of 't1' equivalent to 'a' has been replaced
-                        by 'a' resulting in 't2'. *)
-    Inductive Replaced: A -> T -> T -> Prop :=
-    | replaced_root:
-        forall x a b t1 t2,
-          Equivalent x a ->
-          Replaced x (node b a t1 t2) (node b x t1 t2)
-    | replaced_left:
-        forall x t1 t2 b a t,
-          Replaced x t1 t2 ->
-          Replaced x (node b a t1 t) (node b a t2 t)
-    | replaced_right:
-        forall x t1 t2 b a t,
-          Replaced x t1 t2 ->
-          Replaced x (node b a t t1) (node b a t t2).
-
-    Definition Avl (t:T): Prop :=
-      match is_node t with
-      | left  p => Balanced (height t) (balance t) t
-                   /\
-                   Sorted (least t p) (greatest t p) t
-      | right _ => True
-      end.
-
-    Fixpoint inorder (t:T): List.L :=
-      match t with
-        empty => []
-      | node b a t1 t2 => inorder t1 ++ a :: inorder t2
-      end.
-
-  End draft.
-End Make2.
